The proof is working + Removed the record from proofs

Rsp.fst
@@ -4,10 +4,11 @@ open FStar.Calc
 open FStar.Tactics
 
 open Common
+
+open IO.Behavior
 open IOStHist
 open M4
 open Minterop
-open IO.Behavior
 
 noeq type compiler = {
   interface : Type;
@@ -38,16 +39,6 @@ noeq type compiler = {
   compile_whole : (#i:interface) -> (#pi:monitorable_prop) -> whole_s i pi -> Tot (whole_t i);
 }
   
-let rsp (op:compiler) (i:op.interface) (pi:op.monitorable_prop) (ps:op.prog_s i pi) : Type0 =
-  (forall cs. op.beh_s (cs `op.link_s` ps) `op.included_in_s` (op.safety_prop pi))
-  ==> (forall (ct: op.ctx_t i). (
-      let pt = op.compile_prog ps in
-      op.beh_t (ct `op.link_t` pt) `op.included_in_t` (op.safety_prop pi)))
-
-let tp (op:compiler) (i:op.interface) (pi:op.monitorable_prop) (ws:op.whole_s i pi) : Type0 =
-    ((op.beh_s ws `op.included_in_s` (op.safety_prop pi)) ==>  
-      (op.beh_t (op.compile_whole ws) `op.included_in_t` (op.safety_prop pi)))
-
 noeq type interface = {
   a : Type;  ad : exportable a;
   b : Type;  bd : ml b;         // b has to be importable and exportable
@@ -56,21 +47,24 @@ noeq type interface = {
   cpost : checkable4 post;
 }
 
-type whole_s (i:interface) (pi:check_type) = unit -> M4wp i.c pi (fun _ _ _ -> True)
+let monitorable_prop = check_type
+let safety_prop = pi_to_set
+
+type whole_s (i:interface) (pi:monitorable_prop) = unit -> M4wp i.c pi (fun _ _ _ -> True)
 type whole_t (i:interface) = unit -> M4 i.cd.etype
 
-type ctx_s (i:interface) (pi:check_type) = (x:i.a) -> M4wp i.b pi (i.post x)
-type ctx_p (i:interface) (pi:check_type) = i.ad.etype -> M4wp i.b pi (fun _ _ _ -> True)
+type ctx_s (i:interface) (pi:monitorable_prop) = (x:i.a) -> M4wp i.b pi (i.post x)
+type ctx_p (i:interface) (pi:monitorable_prop) = i.ad.etype -> M4wp i.b pi (fun _ _ _ -> True)
 type ctx_t (i:interface) = i.ad.etype -> M4 i.b
 
-type prog_s (i:interface) (pi:check_type) = ctx_s i pi -> M4wp i.c pi (fun _ _ _ -> True)
-type prog_t (i:interface) (pi:check_type) = ctx_p i pi -> M4 i.cd.etype
+type prog_s (i:interface) (pi:monitorable_prop) = ctx_s i pi -> M4wp i.c pi (fun _ _ _ -> True)
+type prog_t (i:interface) (pi:monitorable_prop) = ctx_p i pi -> M4 i.cd.etype
 
 unfold 
 let beh_s 
   #a
   #b
-  (pi:check_type) 
+  (pi:monitorable_prop) 
   (ws:(x:a -> M4wp b pi (fun _ _ _ -> True))) 
   (x:a) =
   behavior (reify (ws x) (gio_post pi []) [])
@@ -79,7 +73,7 @@ unfold
 let beh_t #a #b (wt:a -> M4 b) (x:a) =
   behavior (reify (wt x) (fun _ -> True))
 
-let rec handle #t2 (tree : io (t2)) (pi:check_type) : M4wp t2 pi (fun _ _ _ -> True) = begin
+let rec handle #t2 (tree : io (t2)) (pi:monitorable_prop) : M4wp t2 pi (fun _ _ _ -> True) = begin
   match tree with
   | Return r -> r 
   | Throw r -> IOStHist.throw r
@@ -103,7 +97,7 @@ let extract_local_events (s0 s1:events_trace) :
 
 let ctx_p_to_ctx_s
   (i  : interface)
-  (pi : check_type)
+  (pi : monitorable_prop)
   (cp  : ctx_p i pi) : 
   Tot (ctx_s i pi) =
   fun (x:i.a) -> 
@@ -120,20 +114,42 @@ let ctx_p_to_ctx_s
 
 let ctx_t_to_ctx_p
   (i  : interface)
-  (pi : check_type)
+  (pi : monitorable_prop)
   (ct : ctx_t i) :
   Tot (ctx_p i pi) =
   fun (x:i.ad.etype) -> handle (reify (ct x) (fun _ -> True)) pi
 
-let export_prog_s
-  (i  : interface)
-  (pi : check_type)
+let compile_prog
+  (#i  : interface)
+  (#pi : monitorable_prop)
   (f  : prog_s i pi) : 
   Tot (prog_t i pi) =
     (fun (ct:ctx_p i pi) ->
       let cs = ctx_p_to_ctx_s i pi ct in
       let tree : io (events_trace * i.c) = reify (f cs) (gio_post pi []) [] in
-      export (MFOUR?.reflect (fun _ -> iost_to_io tree) <: MFOUR i.c (fun p -> forall res. p res)))
+      export (M4?.reflect (fun _ -> iost_to_io tree) <: MFOUR i.c (fun p -> forall res. p res)))
+
+let compile_whole 
+  (#i  : interface)
+  (#pi : monitorable_prop)
+  (f  : whole_s i pi) : 
+  Tot (whole_t i) =
+    (fun _ ->
+      let tree : io (events_trace * i.c) = reify (f ()) (gio_post pi []) [] in
+      export (M4?.reflect (fun _ -> iost_to_io tree) <: MFOUR i.c (fun p -> forall res. p res)))
+ 
+val link_s  : (#i:interface) -> (#pi:check_type) -> ctx_s i pi -> prog_s i pi -> Tot (whole_s i pi)
+let link_s = (fun #i #pi c p -> (fun _ -> p c))
+
+val link_t  : (#i:interface) -> (#pi:check_type) -> ctx_t i -> prog_t i pi -> Tot (whole_t i)
+let link_t #i #pi c p : whole_t i = (fun _ -> p (ctx_t_to_ctx_p i pi c))
+  
+let res_s   = (fun i -> maybe (events_trace * i.c))
+let res_t   = (fun i -> maybe (i.cd.etype))
+  
+val included_in_s : (#i:interface) -> set_of_traces (res_s i) -> set_of_traces (res_s i) -> Type0
+let included_in_s = (fun (#i:interface) -> included_in #(res_s i) #(res_s i) id)
+let included_in_t = (fun (#i:interface) -> included_in #(maybe i.cd.etype) #(maybe (events_trace * i.c)) (inl_app (compose export cdr)))
 
 let seci : compiler = {
   interface = interface;
@@ -143,144 +159,86 @@ let seci : compiler = {
   set_of_traces = set_of_traces;
 
   res_s   = (fun i -> maybe (events_trace * i.c));
-  prog_s  = (fun i pi -> prog_s i pi);
-  ctx_s   = (fun i pi -> ctx_s i pi);
-  whole_s = (fun i pi -> whole_s i pi);
+  prog_s  = prog_s;
+  ctx_s   = ctx_s;
+  whole_s = whole_s;
   
-  link_s = (fun #i #pi c p -> (fun _ -> p c) <: whole_s i pi);
+  link_s = link_s;
 
   res_t   = (fun i -> maybe (i.cd.etype));
-  prog_t  = (fun i pi -> prog_t i pi);
-  ctx_t   = (fun i -> ctx_t i);
-  whole_t = (fun i -> whole_t i);
-  link_t = (fun #i #pi c p -> (fun _ -> p (ctx_t_to_ctx_p i pi c)) <: whole_t i);
+  prog_t  = prog_t;
+  ctx_t   = ctx_t;
+  whole_t = whole_t;
+  link_t = link_t;
 
   beh_s = (fun #i #pi w -> beh_s #unit #i.c pi w ());
   beh_t = (fun #i w -> beh_t #unit #i.cd.etype w ());
   
-  included_in_s = (fun #i -> included_in id);
-  included_in_t = (fun #i -> included_in #(maybe i.cd.etype) #(maybe (events_trace * i.c)) (inl_app (compose export cdr)));
+  included_in_s = included_in_s;
+  included_in_t = included_in_t;
 
-  compile_prog  = (fun #i #pi -> export_prog_s i pi);
-  compile_whole = (fun #i #pi -> _export_GIO_arrow_spec pi);
+  compile_prog  = compile_prog;
+  compile_whole = compile_whole;
 }
 
-let _export_whole_lemma
-  #t1 {| d1:importable t1 |} 
-  #t2 {| d2:exportable t2 |}
+
+let beh_export_whole
+  (i  : interface)
   (pi : check_type) 
-  (f:(x:t1 -> M4wp t2 pi (fun _ _ _ -> True))) 
-  (x':d1.itype) : 
+  (f  : whole_s i pi) :
   Lemma (
-    let ef : d1.itype -> M4 d2.etype = _export_GIO_arrow_spec pi f in
-    match import x' with
-    | Some x -> (
-       beh_t ef x' `included_in (inl_app (compose export cdr))` beh_s pi f x)
-    | None -> beh_t ef x' `included_in id` empty_set ()) =
-
-  let ef : d1.itype -> M4 d2.etype = _export_GIO_arrow_spec pi f in
-  let included_in_id #a = included_in #a #a (id #a) in
-  match import x' with
-  | Some x -> begin
-    let l = reify (ef x') (fun _ -> True) in
-    let __ll : unit -> MFOUR d2.etype (fun p -> forall res. p res) = (fun _ -> 
-            let tree : io (events_trace * t2) = reify (f x) (gio_post pi []) [] in
-            export (MFOUR?.reflect (fun _ -> iost_to_io tree) <: MFOUR t2 (fun p -> forall res. p res))) in
-    let ll = reify (__ll ()) (fun _ -> True) in
-    // TODO: Cezar: The idea behind this is to get rid of the `match`  
-    // because we did it already in the proof.
-    // Related github issues: https://github.com/FStarLang/FStar/issues/2169
-    assert (l == ll) by (
-      unfold_def (`_export_GIO_arrow_spec);
-      let xkkk = (match (List.Tot.nth (cur_binders ()) 12) with
-      | Some y -> y | None -> fail "asdf") in
-      // l_to_r [`xkkk];
-      tadmit ()//;
-      // dump "h"
-    );
-    assert (behavior l `included_in_id` behavior ll);
-
-    calc (included_in_id) {
-        behavior ll;
-        `included_in_id` {}
-        behavior (reify (
-            (export (MFOUR?.reflect (ref (iost_to_io (reify (f x) (gio_post pi []) []))) <: MFOUR t2 (fun p -> forall res. p res)) <: d2.etype)) (fun _ -> True));
-        // TODO: Cezar: this should be just an unfolding of `reify`. I talked with Guido
-        // and it seems using tactics is not a solution to unfold `reify` for 
-        // layered effects because: "reification of layered effects is explicitly disabled
-        // since it requires producing the indices for the bind, and we do not store them
-        // anywhere". I tried to manually unfold looking at EMF* (Dijkstra Monads for
-        // Free), but it seems that F* does not accept this proof. I created a new file only
-        // for this problem: `UnfoldReify.fst`.
-        // Related github issue: https://github.com/FStarLang/FStar/issues/2163
-        `included_in_id` { admit () }
-        // TODO: Cezar: is the 3rd argument correct? I suppose it should use pre and post
-        behavior (M4.ibind t2 d2.etype (fun p -> forall res. p res) (fun x -> m4_return_wp (d2.etype) (export x))
-            (reify (MFOUR?.reflect (ref (iost_to_io (reify (f x) (gio_post pi []) []))) <: MFOUR t2 (fun p -> forall res. p res)))
-            (fun x -> lift_pure_mfour d2.etype (fun p -> p (export x)) (fun _ -> export x)) (fun _ -> True));
-    };
-
-    beh_included_bind_tot #t2 #d2.etype
-        (reify (MFOUR?.reflect (ref (iost_to_io (reify (f x) (gio_post pi []) []))) <: MFOUR t2 (fun p -> forall res. p res)) (compute_post t2 (Mkexportable?.etype d2) (fun x -> m4_return_wp (Mkexportable?.etype d2) (export x)) (fun _ -> True)))
-        export;
-
-    assert (
-        (behavior (M4.ibind t2 d2.etype (fun p -> forall res. p res) (fun x -> m4_return_wp (d2.etype) (export x))
-            (reify (MFOUR?.reflect (ref (iost_to_io (reify (f x) (gio_post pi []) []))) <: MFOUR t2 (fun p -> forall res. p res)))
-            (fun x -> lift_pure_mfour d2.etype (fun p -> p (export x)) (fun _ -> export x)) (fun _ -> True)))
-        `included_in (inl_app export)`
-        (behavior (reify (MFOUR?.reflect (ref (iost_to_io (reify (f x) (gio_post pi []) []))) <: MFOUR t2 (fun p -> forall res. p res)) (fun _ -> True)))
-    ) by (unfold_def (`ibind));
-
-    calc (included_in_id) {
-        behavior (reify (MFOUR?.reflect (ref (iost_to_io (reify (f x) (gio_post pi []) []))) <: MFOUR t2 (fun p -> forall res. p res)) (fun _ -> True));
-        `included_in_id` {}
-        behavior (iost_to_io (reify (f x) (gio_post pi []) []));
-    };
-
-    beh_iost_to_io t2 (reify (f x) (gio_post pi []) []);
-
-    assert (
-        behavior (iost_to_io (reify (f x) (gio_post pi []) []))
-        `included_in (inl_app cdr)` 
-        beh_s pi f x)
-  end
-  | None -> begin
-    calc (==) {
-        reify (ef x') (fun _ -> True);
-        == {}
-        reify ((_export_GIO_arrow_spec pi f <: (d1.itype -> M4 d2.etype)) x') (fun _ -> True);
-        // TODO: Cezar: two admits here.
-        == { 
-          _ by (unfold_def(`_export_IOStHist_arrow_spec); norm [iota]; tadmit ()) }
-        reify (M4.raise Contract_failure) (fun _ -> True);
-        == { admit () }
-        Throw Contract_failure;
-    }
-  end
-
-let export_whole_lemma 
-  #t1 {| d1:importable t1 |} 
-  #t2 {| d2:exportable t2 |}
-  (pi:check_type)
-  (f:(x:t1 -> M4wp t2 pi (fun _ _ _ -> True))) : 
-  Lemma (forall (x':d1.itype). (
-    let ef : d1.itype -> M4 d2.etype = export f in
-    match import x' with
-    | Some x -> (
-        beh_t ef x' `included_in (inl_app (compose export cdr))` beh_s pi f x)
-    | None ->  beh_t ef x' `included_in id` empty_set ())) =
-  admit ();
-  Classical.forall_intro (_export_whole_lemma pi f)
-
-let beh_export_unit_whole_lemma
-  #t2 {| d2:exportable t2 |}
-  (pi:check_type)
-  (f:(unit -> M4wp t2 pi (fun _ _ _ -> True))) : 
-  Lemma (
-    let ef : unit -> M4 d2.etype = _export_GIO_arrow_spec pi f in
+    let ef : whole_t i = compile_whole f in
     beh_t ef () `included_in (inl_app (compose export cdr))` beh_s pi f ()) =
-  _export_whole_lemma pi f ()
+
+  let ef : whole_t i = compile_whole f in
+  let included_in_id #a = included_in #a #a (id #a) in
+  let l1 = reify (ef ()) (fun _ -> True) in
+
+  let l2 = reify (
+          (export (M4?.reflect (ref (iost_to_io (reify (f ()) (gio_post pi []) []))) <: MFOUR i.c (fun p -> forall res. p res)) <: i.cd.etype)) (fun _ -> True) in 
+
+  let l3s = reify (M4?.reflect (ref (iost_to_io (reify (f ()) (gio_post pi []) []))) <: MFOUR i.c (fun p -> forall res. p res)) in
+  let l3 = (M4.ibind i.c i.cd.etype (fun p -> forall res. p res) (fun x -> m4_return_wp (i.cd.etype) (export x))
+          (l3s)
+          (fun x -> lift_pure_mfour i.cd.etype (fun p -> p (export x)) (fun _ -> export x)) (fun _ -> True)) in
+
+  assert (l1 == l2) by (norm [delta_only [`%compile_whole]]);
+  assert (behavior l1 `included_in id` behavior l2);
+  // TODO: Cezar: this should be just an unfolding of `reify`. I talked with Guido
+  // and it seems using tactics is not a solution to unfold `reify` for 
+  // layered effects because: "reification of layered effects is explicitly disabled
+  // since it requires producing the indices for the bind, and we do not store them
+  // anywhere". I tried to manually unfold looking at EMF* (Dijkstra Monads for
+  // Free), but it seems that F* does not accept this proof. I created a new file only
+  // for this problem: `UnfoldReify.fst`.
+  // Related github issue: https://github.com/FStarLang/FStar/issues/2163
+  // `included_in_id` { admit () }
+  // TODO: Cezar: is the 3rd argument correct? I suppose it should use pre and post
+  // behavior (M4.ibind i.c i.cd.etype (fun p -> forall res. p res) (fun x -> m4_return_wp (i.cd.etype) (export x))
+  assume (behavior l2 `included_in id` behavior l3);
+
+  beh_included_bind_tot #i.c #i.cd.etype
+      (l3s (compute_post i.c (Mkexportable?.etype i.cd) (fun x -> m4_return_wp (Mkexportable?.etype i.cd) (export x)) (fun _ -> True)))
+      export;
+
+  assert (
+      behavior l3
+      `included_in (inl_app export)`
+      behavior (l3s (fun _ -> True))
+  ) by (norm [delta_only [`%ibind]]);
+
+  assert (
+      behavior (l3s (fun _ -> True))
+      `included_in id`
+      behavior (iost_to_io (reify (f ()) (gio_post pi []) []))
+  );
+
+  beh_iost_to_io i.c (reify (f ()) (gio_post pi []) []);
+
+  assert (
+      behavior (iost_to_io (reify (f ()) (gio_post pi []) []))
+      `included_in (inl_app cdr)` 
+      beh_s pi f ())
 
 val import_ctx_t : (#i:interface) -> (#pi:check_type) -> ctx_t i -> ctx_s i pi
 let import_ctx_t #i #pi ct =
@@ -289,125 +247,65 @@ let import_ctx_t #i #pi ct =
 
 let beh_export_ps_ct_in_export_ws
   (i  : interface)
-  (pi : check_type)
+  (pi : monitorable_prop)
   (ps : prog_s i pi)
-  (cp : ctx_p i pi) : 
+  (ct : ctx_t i) : 
   Lemma (
-    let (cs : ctx_s i pi) = ctx_p_to_ctx_s i pi cp in
-    let ws : whole_s i pi = fun _ -> ps cs in
-    let pt : prog_t i pi = export_prog_s i pi ps in
-    let wt : whole_t i = _export_GIO_arrow_spec pi ws in
-    beh_t pt cp `included_in id` beh_t wt ()
+    let (cs : ctx_s i pi) = import_ctx_t #i #pi ct in
+    let ws : whole_s i pi = cs `link_s #i` ps in
+    let pt : prog_t i pi = compile_prog ps in
+    let wt : whole_t i = compile_whole #i #pi ws in
+    beh_t (ct `link_t` pt) () `included_in id` beh_t wt ()
   ) = 
+  let cp = ctx_t_to_ctx_p i pi ct in
   let (cs : ctx_s i pi) = ctx_p_to_ctx_s i pi cp in
-  let ws : whole_s i pi = fun _ -> ps cs in
-  let pt : prog_t i pi = export_prog_s i pi ps in
-  let wt : whole_t i = _export_GIO_arrow_spec pi ws in
-  
-  let included_in_id #a = included_in #a #a (id #a) in
-  // assert (import () == Some ());
-  // TODO: apply l_to_r for: import () == Some ()
-  //       apply l_to_r for: import_ctx_t ct == Some b
-  //       Qed.
-  // Related github issue: https://github.com/FStarLang/FStar/issues/2169
+  let ws : whole_s i pi = cs `link_s` ps in
+  let (cs : ctx_s i pi) = ctx_p_to_ctx_s i pi cp in
+  let pt : prog_t i pi = compile_prog ps in
+  let wt : whole_t i = compile_whole ws in
   assert (reify (pt cp) (fun _ -> True) == reify (wt ()) (fun _ -> True)) by (
-    unfold_def (`export_prog_s);
-    unfold_def (`_export_GIO_arrow_spec)
-    // dump "x"
-    // tadmit ()
-  )
+    norm [delta_only [`%compile_prog]];
+    norm [delta_only [`%compile_whole]];
+    norm [delta_only [`%link_s]]
+  );
+  assert (
+    beh_t (ct `link_t #i #pi` pt) ()
+      `included_in id`
+    beh_t ((fun _ -> pt cp) <: whole_t i) ()) 
+  by (norm [delta_only [`%link_t]])
 
 let seci_rsp_0
-  (i   : seci.interface)
-  (pi  : seci.monitorable_prop)
-  (ps  : seci.prog_s i pi)
-  (ct  : seci.ctx_t i) :
+  (i   : interface)
+  (pi  : monitorable_prop)
+  (ps  : prog_s i pi)
+  (ct  : ctx_t i) :
   Lemma (
-  (forall (cs:seci.ctx_s i pi). 
-    (seci.beh_s #i #pi (cs `seci.link_s #i #pi` ps)) `seci.included_in_s #i` (seci.safety_prop pi))
+  (forall (cs:ctx_s i pi). 
+    (beh_s pi (cs `link_s` ps) ()) `included_in_s` (safety_prop pi))
   ==>  (
-      let pt = seci.compile_prog #i ps in
-      seci.beh_t #i (ct `seci.link_t #i #pi` pt) `seci.included_in_t #i` (seci.safety_prop pi))) =
-  admit ();
+      let pt = compile_prog #i ps in
+      beh_t (ct `link_t #i #pi` pt) () `included_in_t` (safety_prop pi))) =
   let (cp:ctx_p i pi) = ctx_t_to_ctx_p i pi ct in
-  let (cs:seci.ctx_s i pi) = ctx_p_to_ctx_s i pi cp in
-  let ws : seci.whole_s i pi = seci.link_s #i #pi cs ps in
-  assert (seci.beh_s #i #pi ws `seci.included_in_s #i` (seci.safety_prop pi));
-  beh_export_unit_whole_lemma #i.c #i.cd pi ws; // Beh (export ws ()) in Beh (ws ())
-  beh_export_ps_ct_in_export_ws i pi ps cp // Beh ((export ps) ct) in Beh (export ws ())
+  let (cs:ctx_s i pi) = ctx_p_to_ctx_s i pi cp in
+  let ws : whole_s i pi = link_s cs ps in
+  beh_gio_in_pi _ _ pi ws (); // Beh (ws ()) in pi
+  beh_export_whole i pi ws; // Beh (export ws ()) in Beh (ws ())
+  beh_export_ps_ct_in_export_ws i pi ps ct // Beh ((export ps) ct) in Beh (export ws ())
 
-let seci_rsp
-  (i  : seci.interface)
-  (pi : seci.monitorable_prop)
-  (ps : seci.prog_s i pi) :
-  Lemma (rsp seci i pi ps) =
-    Classical.forall_intro (seci_rsp_0 i pi ps)
+let rsp (i:interface) (pi:monitorable_prop) (ps:prog_s i pi) : Type0 =
+  (forall cs. beh_s pi (cs `link_s` ps) () `included_in_s` (safety_prop (pi)))
+  ==> (forall (ct: ctx_t i). (
+      let pt = compile_prog ps in
+      beh_t (ct `link_t` pt) () `included_in_t` (safety_prop (pi))))
+
+let seci_respects_rsp () :
+  Lemma (forall i pi ps. rsp i pi ps) =
+    Classical.forall_intro_4 (seci_rsp_0)
   
-
-// let rsp_premise
-//   (i:interface)
-//   (pi : check_type)
-//   (ps : prog_s i pi)
-//   (ct : ctx_t i) :
-//   Lemma (
-//     let (cs : ctx_s i pi) = import_ctx_t ct in
-//     beh_s pi ps cs `included_in id` (pi_to_set pi)) =
-//   let (cs : ctx_s i pi) = import_ctx_t ct in
-//   beh_gio_in_pi (ctx_s i pi) i.c pi ps cs
-    
-// let rsp_conclusion 
-//   (i  : interface)
-//   (pi : check_type)
-//   (ps : prog_s pi i)
-//   (ct : ctx_t i) :
-//   Lemma (
-//     let pt : prog_t i = export_prog_s i pi ps in
-//     beh_t pt ct `included_in #_ #(maybe (events_trace * i.c)) (inl_app (compose export cdr))` (pi_to_set pi)) = 
-//   let Some (cs : ctx_s pi i) = import_ctx_t ct in
-//   let ws : whole_s pi i = fun _ -> ps cs in
-//   beh_gio_in_pi unit i.c pi ws (); // Beh (ws ()) in pi
-//   beh_export_unit_GIO_lemma #i.c #i.cd pi ws; // Beh (export ws ()) in Beh (ws ())
-//   beh_export_ps_ct_in_export_ws i pi ps ct // Beh ((export ps) ct) in Beh (export ws ())
-
-// let rsp_variant
-//   (i  : interface)
-//   (pi : check_type)
-//   (ps : prog_s pi i)
-//   (ct : ctx_t i) :
-//   Lemma(
-//     (forall (cs:(ctx_s pi i)). beh_s pi ps cs `included_in id` (pi_to_set pi)) 
-//     ==> 
-//     (let pt : prog_t i = export_prog_s i pi ps in
-//      beh_t pt ct `included_in #_ #(maybe (events_trace * i.c)) (inl_app (compose export cdr))` (pi_to_set pi))) = 
-//   rsp_conclusion i pi ps ct
-
-
-// let si = secure_interop
- 
-// let rsp_lemma
-//   (pi : check_type)
-//   (i  : (si pi).source.interface)
-//   (ps : (si pi).source.prog i) :
-//   Lemma (forall pi_set. rsp (secure_interop pi) i ps pi_set) =
-//     Classical.forall_intro_2 (rsp_simple_linking'' pi i ps)
+let tp (i:interface) (pi:monitorable_prop) (ws:whole_s i pi) : Type0 =
+    ((beh_s pi ws () `included_in_s` (safety_prop pi)) ==>  
+      (beh_t (compile_whole ws) () `included_in_t` (safety_prop pi)))
   
-// let tp_lemma
-//   (pi : check_type)
-//   (i : (si pi).source.interface)
-//   (ws : (si pi).source.whole i) : 
-//   Lemma (forall pi_set. tp (si pi) (i) (ws) pi_set)  = 
-//   beh_export_unit_GIO_lemma #i.c #i.cd pi ws
-
-// let secure_linker_respects_rsp () : 
-//   Lemma (forall pi i ps pi_set. rsp (secure_interop pi) i ps pi_set)
-//   by (
-//     unfold_def(`rsp);
-//     explode ();
-//     rewrite_lemma 2 3;
-//     norm [iota]
-//   ) =
-//   Classical.forall_intro_3 (rsp_lemma)
-  
-// let secure_linker_respects_tp () :
-//   Lemma (forall pi i ws pi_set. tp (si pi) i ws pi_set) = 
-//     Classical.forall_intro_3 tp_lemma
+let seci_respects_tp () :
+  Lemma (forall pi i ws. tp i pi ws) = 
+    Classical.forall_intro_3 beh_export_whole
